ironfleet/src/Dafny/Distributed/Protocol/RSL/FailureProof/TopLevel/FailureProof.i.dfy
@@ -2,6 +2,7 @@ include "../TimestampedRslSystem.i.dfy"
 include "../../CommonProof/Constants.i.dfy"
 
 include "../Failover/FailureDetection_toplevel.i.dfy"
+include "../Phase1/Phase1Proof_toplevel.i.dfy"
 include "../Phase2_PostFail/Phase2Proof_toplevel.i.dfy"
 include "../Common/assumptions.i.dfy"
 
@@ -11,9 +12,12 @@ import opened TimestampedRslSystem_i
 import opened CommonProof__Constants_i
 import opened Common_Assumptions
 
-import FOStg_Def = FailureDetection_defns_i
-import P2Stg_Pf = Rs2Phase2Proof_PostFail_Top  
-import P2Stg_Def = RslPhase2Proof_PostFail_i
+import FO_top = FailureDetection_i
+import FO_def = FailureDetection_defns_i
+import P1_top = RslPhase1Proof_Top  
+import P1_def = RslPhase1Proof_i  
+import P2_top = RslPhase2Proof_PostFail_Top
+import P2_def = RslPhase2Proof_PostFail_i
 
 /*****************************************************************************************
 *                                      Guarantees                                        *
@@ -26,8 +30,8 @@ predicate PerformanceGuarantee_Final(ts:TimestampedRslState)
 {
     forall pkt | 
         && pkt in ts.undeliveredPackets 
-        && P2Stg_Def.IsNewReplyPacket(ts, pkt)
-    :: TimeLe(pkt.msg.ts, P2Stg_Def.TimeBoundReplyFinal())
+        && IsNewReplyPacket(ts, pkt)
+    :: TimeLe(pkt.msg.ts, P2_def.TimeBoundReplyFinal())
 }
 
 
@@ -39,35 +43,54 @@ predicate PerformanceGuarantee_Final(ts:TimestampedRslState)
 predicate RslAssumption(ts:TimestampedRslState, opn:OperationNumber)
 {
     && CommonAssumptions(ts)
-    && (InPhase2Stage(ts) ==> P2Stg_Def.RslAssumption(ts, opn))
-    && (InFailoverStage(ts) ==> FOStg_Def.RslAssumption(ts))
+    && (FO_def.FOAssumption(ts))
+    && (InPhase1(ts) ==> P1_def.P1Assumption(ts))
+    && (InPhase2(ts) ==> P2_def.P2Assumption(ts, opn))
+    
 }
 
 predicate RslAssumption2(ts:TimestampedRslState, ts':TimestampedRslState)
+    requires |ts.t_replicas| > 2 && |ts'.t_replicas| > 2
 {
-    (InFailoverStage(ts) && InFailoverStage(ts') ==> FOStg_Def.RslAssumption2(ts, ts'))
+    (InFailover(ts) && InFailover(ts') ==> FO_def.FOAssumption2(ts, ts'))
 }
 
 
 
 /*****************************************************************************************
-*                                     Invariants                                        *
+*                                Main Theorem Proof                                      *
 *****************************************************************************************/
 
 
-// // Main invariant 
-// predicate RslPerfInvariant(ts:TimestampedRslState, opn:OperationNumber) 
-//     requires |ts.t_replicas| > 2
-// {
-//     && RslConsistency(ts)
-//     && AlwaysInvariant(ts, opn)
-//     && PerformanceGuarantee(ts, opn)
-//     && PacketsBallotInvariant(ts)
-//     && (|| Before_2a_Sent_Invariant(ts, opn)
-//         || Before_2b_Sent_Invariant(ts, opn)
-//         || After_2b_Sent_Invariant(ts, opn)
-//     )
-// }
+lemma RSLTopLevel(tglb:seq<TimestampedRslState>, opn:OperationNumber)
+    requires |tglb| > 0
+    requires exists con :: ValidTimestampedRSLBehavior(con, tglb)
+    requires forall i | 0 <= i < |tglb| :: RslAssumption(tglb[i], opn)
+    ensures forall j | 0 <= j < |tglb| :: PerformanceGuarantee_Final(tglb[j])
+{
+    var P1_idx := FO_top.FailoverTopLevel(tglb);
+
+    if P1_idx >= |tglb| {
+        assert forall i | 0 <= i < |tglb| :: |tglb[i].t_replicas| > 2;
+        assert forall i | 0 <= i < |tglb| :: PerformanceGuarantee_Final(tglb[i]);  
+    } else {
+        assert forall i | 0 <= i < P1_idx :: |tglb[i].t_replicas| > 2;
+        assert forall i | 0 <= i < P1_idx :: PerformanceGuarantee_Final(tglb[i]);
+        
+        assume false;
+        var P2_idx := P1_top.Phase1TopLevel(tglb[P1_idx..], opn);
+        if P2_idx >= |tglb| {
+            assert forall i | 0 <= i < |tglb| :: |tglb[i].t_replicas| > 2;
+            assert forall i | 0 <= i < |tglb| :: PerformanceGuarantee_Final(tglb[i]);  
+        } else {
+            assert forall i | 0 <= i < P2_idx :: |tglb[i].t_replicas| > 2;
+            assert forall i | 0 <= i < P2_idx :: PerformanceGuarantee_Final(tglb[i]);  
+
+            P2_top.Phase2TopLevel(tglb[P2_idx..], opn);
+            assert forall i | 0 <= i < |tglb| :: PerformanceGuarantee_Final(tglb[i]);
+        }
+    }
+}
 
 
 /*****************************************************************************************
@@ -77,20 +100,20 @@ predicate RslAssumption2(ts:TimestampedRslState, ts':TimestampedRslState)
 
 
 
-predicate InFailoverStage(ts:TimestampedRslState) 
+predicate InFailover(ts:TimestampedRslState) 
     requires |ts.t_replicas| > 2
 {
     ts.t_replicas[1].v.replica.proposer.election_state.current_view == Ballot(1,0)
 }
 
-predicate InPhase1Stage(ts:TimestampedRslState) 
+predicate InPhase1(ts:TimestampedRslState) 
     requires |ts.t_replicas| > 2
 {
     && ts.t_replicas[1].v.replica.proposer.election_state.current_view == Ballot(1,1)
     && ts.t_replicas[1].v.replica.proposer.current_state != 2
 }
 
-predicate InPhase2Stage(ts:TimestampedRslState) 
+predicate InPhase2(ts:TimestampedRslState) 
     requires |ts.t_replicas| > 2
 {
     && ts.t_replicas[1].v.replica.proposer.election_state.current_view == Ballot(1,1)
