ironfleet/src/Dafny/Distributed/Protocol/RSL/FailureProof/Phase1/Phase1Proof_toplevel.i.dfy
@@ -75,16 +75,18 @@ predicate ExistingPacketsBallotOpn(ts:TimestampedRslState, opn:OperationNumber) 
 // Main invariant 
 predicate Phase1Invariant(ts:TimestampedRslState, opn:OperationNumber) 
     requires |ts.t_replicas| > 2
+    requires RslConsistency(ts)
 {
     && AlwaysInvariant(ts, opn)
-    && true // TODO
+    && forall pkt | pkt in ts.t_environment.sentPackets :: !IsNewReplyPacket(ts, pkt)
+    && true // add more stuff
 }
 
 
 
 lemma Phase1TopLevel(tglb:seq<TimestampedRslState>, opn:OperationNumber) returns (startPhase2Idx:int)
-    requires exists con :: ValidTimestampedRSLBehavior(con, tglb)
     requires forall i | 0 <= i < |tglb| :: P1Assumption(tglb[i])
+    requires forall i | 0 < i < |tglb| :: TimestampedRslNext(tglb[i - 1], tglb[i])
     // Phase1 lasts up till right before startPhase2Idx
     // startPhase2Idx is the initial state of phase 2
     ensures forall j | 0 <= j < |tglb| && j < startPhase2Idx :: Phase1Invariant(tglb[j], opn)
